@prefix : <http://www.coolfutures.net/rdf/2021/bibannotation#> .
@prefix owl: <http://www.w3.org/2002/07/owl#> .
@prefix rdf: <http://www.w3.org/1999/02/22-rdf-syntax-ns#> .
@prefix xml: <http://www.w3.org/XML/1998/namespace> .
@prefix xsd: <http://www.w3.org/2001/XMLSchema#> .
@prefix rdfs: <http://www.w3.org/2000/01/rdf-schema#> .
@base <http://www.coolfutures.net/rdf/2021/bibannotation#> .

<http://www.coolfutures.net/rdf/2021/bibannotation#> rdf:type owl:Ontology ;
                                                      <http://purl.org/dc/elements/1.1/creator> "Peter Reimann"@en ;
                                                      rdfs:comment "A simple annotation ontology for biobliographic references"@en ;
                                                      rdfs:seeAlso "https://www.w3.org/2001/Annotea/Papers/www10/annotea-www10.html"@en .

#################################################################
#    Annotation properties
#################################################################

###  http://purl.org/dc/elements/1.1/creator
<http://purl.org/dc/elements/1.1/creator> rdf:type owl:AnnotationProperty .


#################################################################
#    Object Properties
#################################################################

###  http://purl.org/dc/elements/1.1/creator
<http://purl.org/dc/elements/1.1/creator> rdf:type owl:ObjectProperty .


###  http://www.coolfutures.net/rdf/2021/bibannotation#annotates
:annotates rdf:type owl:ObjectProperty ;
           rdfs:comment ""@en ,
                        "The relation between an annotation resource and the resource to which the annotation applies." .


###  http://www.coolfutures.net/rdf/2021/bibannotation#body
:body rdf:type owl:ObjectProperty ;
      rdfs:comment "The content of the annotation."@en .


###  http://www.coolfutures.net/rdf/2021/bibannotation#context
:context rdf:type owl:ObjectProperty ;
         rdfs:comment """Context is tricky for bibliographic references because there is no way to describe a location of a published document with precision. One way that is workable is to use as the object of the context predicate a blank node and provide in the blank node as much information as possible. For instance: 

anno:context [
    rdf:value \"The namespaces for these additional types are specified to Amaya in a local configuration file that is read at startup. Amaya will use the namespace name to try to retrieve an RDF schema from the Web or the schema content can be cached in a local file and specified with the same startup configuration.\" ; 
     :startpage 56 ; 
     :section deo:methods ]

in this format, the rdf:value holds a quote and the other predicates provide meta-data on the quote. The deo ontology is useful to describe the part of the resource where the quote comes from. 

The simplest way is of course to just add a descriptive string, e.g.:

anno:context \"page 56, 2nd paragraph\" or such."""@en ,
                      "Context within the resource named in annotates to which the annotation most directly applies."@en ;
         rdfs:seeAlso "https://sparontologies.github.io/deo/current/deo.html#d4e270"^^xsd:anyURI .


###  http://www.coolfutures.net/rdf/2021/bibannotation#related
:related rdf:type owl:ObjectProperty ;
         rdfs:comment "A relation between an annotation and a (collection of) resource(s) that augment the resource that is the body of the annotation. This may point to related issues, discussion threads, etc."@en .


#################################################################
#    Data properties
#################################################################

###  http://purl.org/dc/elements/1.1/date
<http://purl.org/dc/elements/1.1/date> rdf:type owl:DatatypeProperty ;
                                       rdfs:comment "The date and time on which the annotation was last modified."@en .


###  http://www.coolfutures.net/rdf/2021/bibannotation#created
:created rdf:type owl:DatatypeProperty ;
         rdfs:comment "The date and time on which the annotation was created"@en .


#################################################################
#    Classes
#################################################################

###  http://www.coolfutures.net/rdf/2021/bibannotation#Advice
:Advice rdf:type owl:Class ;
        rdfs:subClassOf :BibAnnotation ;
        rdfs:comment "A subclass of Annotation representing advice to the reader.Different Suggestion as the suggestion addresses mor the writer, or the annotator themselves."@en .


###  http://www.coolfutures.net/rdf/2021/bibannotation#BibAnnotation
:BibAnnotation rdf:type owl:Class .


###  http://www.coolfutures.net/rdf/2021/bibannotation#Change
:Change rdf:type owl:Class ;
        rdfs:subClassOf :Suggestion ;
        rdfs:comment "A subclass of Annotation describing annotations that document or propose a change to the source document."@en .


###  http://www.coolfutures.net/rdf/2021/bibannotation#Comment
:Comment rdf:type owl:Class ;
         rdfs:subClassOf :BibAnnotation ;
         rdfs:comment "A subclass of Annotation describing annotations that are comments."@en .


###  http://www.coolfutures.net/rdf/2021/bibannotation#Example
:Example rdf:type owl:Class ;
         rdfs:subClassOf :BibAnnotation ;
         rdfs:comment "A subclass of Annotation representing examples."@en .


###  http://www.coolfutures.net/rdf/2021/bibannotation#Explanation
:Explanation rdf:type owl:Class ;
             rdfs:subClassOf :BibAnnotation ;
             rdfs:comment "A subclass of Annotation representing explanations of content."@en .


###  http://www.coolfutures.net/rdf/2021/bibannotation#Question
:Question rdf:type owl:Class ;
          rdfs:subClassOf :BibAnnotation ;
          rdfs:comment "A subclass of Annotation representing questions about the content."@en .


###  http://www.coolfutures.net/rdf/2021/bibannotation#SeeAlso
:SeeAlso rdf:type owl:Class ;
         rdfs:subClassOf :BibAnnotation ;
         rdfs:comment "A subclass of Annotation representing a reference to another resource."@en .


###  http://www.coolfutures.net/rdf/2021/bibannotation#Suggestion
:Suggestion rdf:type owl:Class ;
            rdfs:subClassOf :BibAnnotation ;
            rdfs:comment "A subtype of annotation that suggests further lines of research, an improvement, etc."@en .


#################################################################
#    Annotations
#################################################################

<http://purl.org/dc/elements/1.1/creator> rdfs:comment "The creator of the annotation"@en .


###  Generated by the OWL API (version 4.5.9.2019-02-01T07:24:44Z) https://github.com/owlcs/owlapi
