@prefix : <http://www.coolfutures.net/rdf/2021/bibannotation#> .
@prefix owl: <http://www.w3.org/2002/07/owl#> .
@prefix rdf: <http://www.w3.org/1999/02/22-rdf-syntax-ns#> .
@prefix xml: <http://www.w3.org/XML/1998/namespace> .
@prefix xsd: <http://www.w3.org/2001/XMLSchema#> .
@prefix rdfs: <http://www.w3.org/2000/01/rdf-schema#> .
@base <http://www.coolfutures.net/rdf/2021/bibannotation#> .

<http://www.coolfutures.net/rdf/2021/bibannotation#> rdf:type owl:Ontology ;
                                                      <http://purl.org/dc/terms/creator> "Peter Reimann"@en ;
                                                      rdfs:comment "A simple annotation ontology for biobliographic references"@en ;
                                                      rdfs:seeAlso "https://www.w3.org/2001/Annotea/Papers/www10/annotea-www10.html"@en .

#################################################################
#    Annotation properties
#################################################################

###  http://purl.org/dc/terms/creator
<http://purl.org/dc/terms/creator> rdf:type owl:AnnotationProperty .


#################################################################
#    Object Properties
#################################################################

###  http://purl.org/dc/terms/creator
<http://purl.org/dc/terms/creator> rdf:type owl:ObjectProperty .


###  http://purl.org/dc/terms/relation
<http://purl.org/dc/terms/relation> rdf:type owl:ObjectProperty ;
                                    rdfs:comment "A relation between an annotation and a (collection of) resource(s) that augment the resource that is the body of the annotation. This may point to related issues, discussion threads, etc."@en .


###  http://www.coolfutures.net/rdf/2021/bibannotation#annotates
:annotates rdf:type owl:ObjectProperty ;
           rdfs:domain :BibAnnotation ;
           rdfs:comment ""@en ,
                        "X annotes Y." .


###  http://www.coolfutures.net/rdf/2021/bibannotation#body
:body rdf:type owl:ObjectProperty ;
      rdfs:comment "The content of the annotation."@en .


###  http://www.coolfutures.net/rdf/2021/bibannotation#context
:context rdf:type owl:ObjectProperty ;
         rdfs:comment "Context within the resource named in annotates to which the annotation most directly applies."@en ;
         rdfs:seeAlso "https://sparontologies.github.io/deo/current/deo.html"^^xsd:anyURI .


#################################################################
#    Data properties
#################################################################

###  http://purl.org/dc/elements/1.1/date
<http://purl.org/dc/elements/1.1/date> rdf:type owl:DatatypeProperty ;
                                       rdfs:comment "The date and time on which the annotation was last modified."@en .


###  http://www.coolfutures.net/rdf/2021/bibannotation#created
:created rdf:type owl:DatatypeProperty ;
         rdfs:range xsd:dateTime ;
         rdfs:comment "The date and time on which the annotation was created"@en .


#################################################################
#    Classes
#################################################################

###  http://www.coolfutures.net/rdf/2021/bibannotation#Advice
:Advice rdf:type owl:Class ;
        rdfs:subClassOf :BibAnnotation ;
        rdfs:comment "A subclass of Annotation representing advice to the reader.Different Suggestion as the suggestion addresses mor the writer, or the annotator themselves."@en .


###  http://www.coolfutures.net/rdf/2021/bibannotation#BibAnnotation
:BibAnnotation rdf:type owl:Class .


###  http://www.coolfutures.net/rdf/2021/bibannotation#Change
:Change rdf:type owl:Class ;
        rdfs:subClassOf :Suggestion ;
        rdfs:comment "A subclass of Annotation describing annotations that document or propose a change to the source document."@en .


###  http://www.coolfutures.net/rdf/2021/bibannotation#Comment
:Comment rdf:type owl:Class ;
         rdfs:subClassOf :BibAnnotation ;
         rdfs:comment "A subclass of Annotation describing annotations that are comments."@en .


###  http://www.coolfutures.net/rdf/2021/bibannotation#Example
:Example rdf:type owl:Class ;
         rdfs:subClassOf :BibAnnotation ;
         rdfs:comment "A subclass of Annotation representing examples."@en .


###  http://www.coolfutures.net/rdf/2021/bibannotation#Explanation
:Explanation rdf:type owl:Class ;
             rdfs:subClassOf :BibAnnotation ;
             rdfs:comment "A subclass of Annotation representing explanations of content."@en .


###  http://www.coolfutures.net/rdf/2021/bibannotation#Question
:Question rdf:type owl:Class ;
          rdfs:subClassOf :BibAnnotation ;
          rdfs:comment "A subclass of Annotation representing questions about the content."@en .


###  http://www.coolfutures.net/rdf/2021/bibannotation#SeeAlso
:SeeAlso rdf:type owl:Class ;
         rdfs:subClassOf :BibAnnotation ;
         rdfs:comment "A subclass of Annotation representing a reference to another resource."@en .


###  http://www.coolfutures.net/rdf/2021/bibannotation#Suggestion
:Suggestion rdf:type owl:Class ;
            rdfs:subClassOf :BibAnnotation ;
            rdfs:comment "A subtype of annotation that suggests further lines of research, an improvement, etc."@en .


#################################################################
#    Annotations
#################################################################

<http://purl.org/dc/terms/creator> rdfs:comment "The creator of the annotation"@en .


###  Generated by the OWL API (version 4.5.9.2019-02-01T07:24:44Z) https://github.com/owlcs/owlapi
