#################################
# Concepts: Bloom's Learning CognitiveOutcome
#################################

# Definitions from https://en.wikipedia.org/wiki/Bloom%27s_taxonomy

PREFIX : <http://www.learn-web.com/thesauri/bloom_outcomes/>  
PREFIX bloom: <http://www.learn-web.com/thesauri/bloom_outcomes/>
PREFIX skos: <http://www.w3.org/2004/02/skos/core#>

### Concept Scheme

:BloomThesaurus a skos:ConceptScheme ; 
  rdfs:label "Bloom learning outcomes" ;
	dc:title "Bloom learning outcomes " ;
	skos:hasTopConcept :CognitiveOutcome, :AffectiveOutcome, :PsychomotorOutcome .
	
### Concepts 

:CognitiveOutcome a skos:Concept ; 
	skos:inScheme :BloomThesaurus ; 
	skos:prefLabel "Cognitive learning outcome"@en . 
	
:AffectiveOutcome a skos:Concept ; 
	skos:inScheme :BloomThesaurus ; 
	skos:prefLabel "Affective learning outcome"@en . 
	
:PsychomotorOutcome a skos:Concept ; 
	skos:inScheme :BloomThesaurus ; 
	skos:prefLabel "Psychomotoric learning outcome"@en . 
	
### Cognitive learning outcomes 
	
:Knowledge a skos:Concept ; 
	skos:inScheme :BloomThesaurus ; 
	skos:prefLabel "Knowledge outcome"@en ; 
	skos:definition "Knowledge involves recognizing or remembering facts, terms, basic concepts, or answers without necessarily understanding what they mean."@en ;
	skos:broader :CognitiveOutcome . 
	
:Comprehension a skos:Concept ; 
	skos:inScheme :BloomThesaurus ; 
	skos:prefLabel "Comprehension outcome"@en ; 
	skos:definition "Comprehension involves demonstrating an understanding of facts and ideas by organizing, summarizing, translating, generalizing, giving descriptions, and stating the main ideas."@en ;
	skos:broader :CognitiveOutcome . 
	
:Application a skos:Concept ; 
	skos:inScheme :BloomThesaurus ; 
	skos:prefLabel "Application outcome"@en ; 
	skos:definition "Comprehension involves demonstrating an understanding of facts and ideas by organizing, summarizing, translating, generalizing, giving descriptions, and stating the main ideas."@en ;
	skos:broader :CognitiveOutcome . 
	
:Analysis a skos:Concept ; 
	skos:inScheme :BloomThesaurus ; 
	skos:prefLabel "Analysis outcome"@en ; 
	skos:definition "Analysis involves examining and breaking information into component parts, determining how the parts relate to one another, identifying motives or causes, making inferences, and finding evidence to support generalizations."@en ;
	skos:broader :CognitiveOutcome . 
	
:Synthesis a skos:Concept ; 
	skos:inScheme :BloomThesaurus ; 
	skos:prefLabel "Synthesis outcome"@en ; 
	skos:definition "Synthesis involves building a structure or pattern from diverse elements; it also refers to the act of putting parts together to form a whole or bringing pieces of information together to form a new meaning."@en ;
	skos:broader :CognitiveOutcome . 
	
:Evaluation a skos:Concept ; 
	skos:inScheme :BloomThesaurus ; 
	skos:prefLabel "Evaluation outcome"@en ; 
	skos:definition "Evaluation involves presenting and defending opinions by making judgments about information, the validity of ideas, or quality of work based on a set of criteria."@en ;
	skos:broader :CognitiveOutcome . 
	
### Affective learning outcomes 
	
:Receiving a skos:Concept ; 
	skos:inScheme :BloomThesaurus ; 
	skos:prefLabel "Receiving outcome"@en ; 
	skos:definition "The lowest level; the student passively pays attention. Without this level, no learning can occur. Receiving is about the student's memory and recognition as well."@en ;
	skos:broader :AffectiveOutcome . 

:Responding a skos:Concept ; 
	skos:inScheme :BloomThesaurus ; 
	skos:prefLabel "Responding outcome"@en ; 
	skos:definition "The student actively participates in the learning process, not only attends to a stimulus; the student also reacts in some way."@en ;
	skos:broader :AffectiveOutcome . 
	
:Valuing a skos:Concept ; 
	skos:inScheme :BloomThesaurus ; 
	skos:prefLabel "Valuing outcome"@en ; 
	skos:definition "The student attaches a value to an object, phenomenon, or piece of information. The student associates a value or some values to the knowledge they acquired."@en ;
	skos:broader :AffectiveOutcome . 
	
:Organizing a skos:Concept ; 
	skos:inScheme :BloomThesaurus ; 
	skos:prefLabel "Organizing outcome"@en ; 
	skos:definition "The student can put together different values, information, and ideas, and can accommodate them within their own schema; the student is comparing, relating and elaborating on what has been learned."@en ;
	skos:broader :AffectiveOutcome . 
	
:Characterizing a skos:Concept ; 
	skos:inScheme :BloomThesaurus ; 
	skos:prefLabel "Characterizing outcome"@en ; 
	skos:definition "The student at this level tries to build abstract knowledge."@en ;
	skos:broader :AffectiveOutcome . 
